\section{Linear Equations; Method of Integrating Factors}
    A \textbf{first order linear equation} is an equation that is only linearly dependent on $y$. Its general form is
    \begin{equation*}
        \frac{dy}{dt} + p(t)y = g(t) \text{ or } P(t)\frac{dy}{dt} + Q(t)y = G(t)
    \end{equation*}
    Most equations cannot be solved with simple integration, so we can use an \textbf{integrating factor} $\mu(t)$. This works for any first order linear equation. 
    \begin{equation*}
        \frac{dy}{dt} + ay = g(t)
    \end{equation*}
    Now, we need to find a a $\mu(t)$ so that
    \begin{equation*}
        \frac{d\mu}{dt} = a\mu
    \end{equation*}
    which yields $\mu(t) = e^{at}$. Multiplying the original equation by $\mu(t)$
    \begin{equation*}
        e^{at}\frac{dy}{dt} + ae^{at}y = e^{at}g(t)
    \end{equation*}
    or
    \begin{equation*}
        \frac{d}{dt}(e^{at}y) = e^{at}g(t)
    \end{equation*}
    By integrating both sides,
    \begin{equation*}
        e^{at}y = \int e^{at}g(t)dt + c
    \end{equation*}
    \begin{equation*}
        y = e^{-at}\int_{t_0}^te^{as}g(s)ds + ce^{-at}
    \end{equation*}
    Now, let's extend this to the general first order linear equation:
    \begin{equation*}
        \frac{dy}{dt} + p(t)y = g(t)
    \end{equation*}
    Multiply by $\mu(t)$
    \begin{equation*}
        \mu(t)\frac{dy}{dt} + p(t)\mu(t)y = \mu(t)g(t)
    \end{equation*}
    We know that $\frac{d(\mu(t)y)}{dt} = \mu(t)\frac{dy}{dt} + p(t)\mu(t)y$, if
    \begin{equation*}
        \frac{d\mu(t)}{dt} = p(t)\mu(t)
    \end{equation*}
    if $p(t) > 0$
    \begin{equation*}
        \frac{d\mu(t) / dt}{\mu(t)} = p(t)
    \end{equation*}
    \begin{equation*}
        \ln \mu(t) = \int p(t) dt + k
    \end{equation*}
    By choosing $k$ to be 0, we obtain the simplest possible $\mu(t)$
    \begin{equation*}
        \mu(t) = \exp \int p(t) dt
    \end{equation*}
    Now,
    \begin{equation*}
        \frac{d}{dt}[\mu(t)y] = \mu(t)\frac{dy}{dt} + p(t)\mu(t)y = \mu(t)g(t)
    \end{equation*}
    By integrating,
    \begin{equation*}
        \mu(t)y = \int \mu(t)g(t)dt + c
    \end{equation*}
    \begin{equation*}
        y = \frac{1}{\mu(t)}[\int_{t_0}^t \mu(t)g(s)ds + c]
    \end{equation*}
        
        